<?xml version="1.0"?>

<!DOCTYPE rdf:RDF [
    <!ENTITY http "http://" >
    <!ENTITY www "http://www.ArgOWL.org#" >
    <!ENTITY owl "http://www.w3.org/2002/07/owl#" >
    <!ENTITY aif "http://www.arg.tech/aif#" >
    <!ENTITY hevy "http://www.arg.tech/hevy#" >
    <!ENTITY xsd "http://www.w3.org/2001/XMLSchema#" >
    <!ENTITY rdfs "http://www.w3.org/2000/01/rdf-schema#" >
    <!ENTITY rdf "http://www.w3.org/1999/02/22-rdf-syntax-ns#" >
]>

<rdf:RDF xmlns="&http;www.w3.org/2002/07/owl#"
     xml:base="&http;www.arg.tech/hevy"
     xmlns:rdfs="&http;www.w3.org/2000/01/rdf-schema#"
     xmlns:http="http://"
     xmlns:www="&http;www.ArgOWL.org#"
     xmlns:owl="&http;www.w3.org/2002/07/owl#"
     xmlns:xsd="&http;www.w3.org/2001/XMLSchema#"
     xmlns:rdf="&http;www.w3.org/1999/02/22-rdf-syntax-ns#"
     xmlns:aif="&http;www.arg.tech/aif#"
     xmlns:hevy="&http;www.arg.tech/hevy#">
    
    <Ontology rdf:about="&http;www.arg.tech/hevy#">
        <www:createdBy rdf:datatype="&http;www.w3.org/2001/XMLSchema#string">Dimitra Zografistou</www:createdBy>
        <rdfs:comment rdf:datatype="&http;www.w3.org/2001/XMLSchema#string">The Hevy Ontology - Schema specification</rdfs:comment>
        <versionInfo>version 1.0</versionInfo>
    </Ontology>
    
    
    <!-- Class definitions -->
    
    <owl:Class rdf:about="#EventDescription">
        <rdfs:comment>An information node, the content of which is a description of a real world event. </rdfs:comment>
        <rdfs:subClassOf rdf:resource="&http;www.arg.tech/aif#I-node"/>
    </owl:Class>
    
    <rdfs:Class rdf:about="&http;www.arg.tech/aif#L-node">
        <rdfs:comment>Redefinition of L-node so that it becomes subclass of the EventDescription class.</rdfs:comment>
        <rdfs:subClassOf rdf:resource="&http;www.arg.tech/hevy#EventDescription"/>
    </rdfs:Class>
    
    <rdfs:Class rdf:about="&http;www.arg.tech/hevy#Event">
        <rdfs:comment>The real world event. </rdfs:comment>
    </rdfs:Class>
    
    <rdfs:Class rdf:about="&http;www.arg.tech/hevy#LocutionEvent">
        <rdf:comment>The event of a locution's creation</rdf:comment>
        <rdfs:subClassOf rdf:resource="&http;www.arg.tech/hevy#Event"/>
    </rdfs:Class>
    
    
    
    
    <!-- Object properties -->
    
    <!-- describes-->
    <rdf:Property rdf:about="&http;www.arg.tech/hevy#describes">
        <rdfs:comment>  This property captures the transition from a description to a real world event. </rdfs:comment>
        <rdfs:domain rdf:resource="&http;www.arg.tech/hevy#EventDescription"/>
        <rdfs:range rdf:resource="&http;www.arg.tech/hevy#Event"/>
    </rdf:Property>

    <!-- Datatype properties -->
    
    
    <!-- atPlace -->
    <rdf:Property rdf:about="&http;www.arg.tech/hevy#atPlace">
        <rdfs:comment>Answers the question: ”Where did the event happen?” . 
            This property refers to the particular or relative place that an event occurred. It might
            have a name (e.g., “USA”) or might be defined as a relative name to other entity or entities 
            (e.g., “new unincorporated regions between Mexico and USA”). An event can be correlated to more than one places. 
        </rdfs:comment>
        <rdfs:domain rdf:resource="&http;www.arg.tech/hevy#Event"/>
        <rdfs:range rdf:resource="&http;www.w3.org/2001/XMLSchema#string"/>
    </rdf:Property>

    
    <!-- atTime -->
    <rdf:Property rdf:about="&http;www.arg.tech/hevy#atTime">
        <rdfs:comment>Answers the question: “When did the event happen?” by giving an abstract instant or 
            a time interval. This property refers to imposed temporal boundaries (i.e., a time span) at which an event happened.
            Thus, an event can be related to only one time span.
        </rdfs:comment>
        <rdfs:domain rdf:resource="&http;www.arg.tech/hevy#Event"/>
        <rdfs:range rdf:resource= "xsd:dateTime" />
    </rdf:Property>
    
    
    <!-- circa -->
    <rdf:Property rdf:about="&http;www.arg.tech/hevy#circa">
        <rdfs:comment>Describes a temporal relation expressing approximation in time. A time interval that cannot be
            precisely located in calendar dates and clock times (i.e., chronological series to another time span that can be
            precisely located in chronological series)
         </rdfs:comment>
        <rdfs:domain rdf:resource="&http;www.arg.tech/hevy#Event"/>
        <rdfs:range rdf:resource= "xsd:string" />
    </rdf:Property>
    
    
    <!-- illustrate -->
    <rdf:Property rdf:about="&http;www.arg.tech/hevy#illustrate">
        <rdfs:comment>Depicts that an event can be illustrated by something (media object).
         </rdfs:comment>
        <rdfs:domain rdf:resource="&http;www.arg.tech/hevy#Event"/>
        <rdfs:range rdf:resource= "xsd:string" />
    </rdf:Property>
    
    
     <!-- inSpace -->
     <rdf:Property rdf:about="&http;www.arg.tech/hevy#inSpace">
        <rdfs:comment>Refers to an abstract region of space and answers to the question: “Where an event happened?” in
            spatial terms. It refers an event to a region of space (i.e., it only asserts the event occurred somewhere within certain
            region but does not assert that the event has occurred everywhere within the region. 
         </rdfs:comment>
        <rdfs:domain rdf:resource="&http;www.arg.tech/hevy#Event"/>
        <rdfs:range rdf:resource= "xsd:string" />
    </rdf:Property>
    
       
     <!-- involved -->
     <rdf:Property rdf:about="&http;www.arg.tech/hevy#involved">
        <rdfs:comment>A (physical, social or mental) object involved in an event.</rdfs:comment>
        <rdfs:domain rdf:resource="&http;www.arg.tech/hevy#Event"/>
        <rdfs:range rdf:resource= "xsd:string" />
    </rdf:Property>
    
    
     <!-- involvedAgent -->
     <rdf:Property rdf:about="&http;www.arg.tech/hevy#involvedAgent">
        <rdfs:comment>an agent involved in an Event.</rdfs:comment>
        <rdfs:domain rdf:resource="&http;www.arg.tech/hevy#Event"/>
        <rdfs:range rdf:resource= "xsd:string" />
    </rdf:Property>
    
    
</rdf:RDF>